Define optimized generator

theories/Generator.v
@@ -23,7 +23,10 @@ From Coq Require Import
 Import ListNotations.
 
 From SLOT Require Import
-     Foundations.
+     Foundations
+     Commutativity
+     Properties
+     Tactics.
 
 From Hammer Require Import
      Tactics.
@@ -32,20 +35,22 @@ Class Generator TE g :=
   { gen_step : g -> option (g * TE) -> Prop
   }.
 
-Notation "A '~~>' B & C" := (gen_step A (Some (B, C))) (at level 20).
+Open Scope slot_scope.
 
-Notation "A '~~>x'" := (gen_step A None) (at level 20).
+Notation "A '~~>' B & C" := (gen_step A (Some (B, C))) (at level 20) : slot_scope.
+
+Notation "A '~~>x'" := (gen_step A None) (at level 20) : slot_scope.
 
 Section GenEnsemble.
-  (** Generator from an ensemble *)
+  (** Generator as an ensemble *)
   Context {TE G : Type} `{Generator TE G}.
 
   Inductive GenEnsemble (g : G) : @TraceEnsemble TE :=
   | gen_ens_nil :
-      gen_step g None ->
+      g ~~>x ->
       GenEnsemble g []
   | gen_ens_cons : forall g' te t,
-      gen_step g (Some (g', te)) ->
+      g ~~> g' & te ->
       GenEnsemble g' t ->
       GenEnsemble g (te :: t).
 End GenEnsemble.
@@ -74,34 +79,32 @@ Module Empty.
   Qed.
 End Empty.
 
-Module List.
-  Section defn.
-    Context (A : Type).
+Section list_defn.
+  Context (A : Type).
 
-    Let G := list A.
+  Let G := list A.
 
-    Inductive ListGenStep : G -> option (G * A) -> Prop :=
-    | lgen_nil :
-        ListGenStep [] None
-    | lgen_cons : forall te t,
-        ListGenStep (te :: t) (Some (t, te)).
+  Inductive ListGenStep : G -> option (G * A) -> Prop :=
+  | lgen_nil :
+      ListGenStep [] None
+  | lgen_cons : forall te t,
+      ListGenStep (te :: t) (Some (t, te)).
 
-    Global Instance listGenerator : Generator A G :=
-      { gen_step := ListGenStep }.
+  Global Instance listGenerator : Generator A G :=
+    { gen_step := ListGenStep }.
 
-    Lemma list_gen_correct : forall l l',
-        GenEnsemble l l' ->
-        l = l'.
-    Proof.
-      intros.
-      induction H.
-      - now inversion H.
-      - subst. now inversion_clear H.
-    Qed.
-  End defn.
-End List.
+  Lemma list_gen_correct : forall l l',
+      GenEnsemble l l' ->
+      l = l'.
+  Proof.
+    intros.
+    induction H.
+    - now inversion H.
+    - subst. now inversion_clear H.
+  Qed.
+End list_defn.
 
-Module Process.
+Section process.
   Section defn.
     Context {Request : Type} {Reply : Request -> Type}.
 
@@ -111,7 +114,7 @@ Module Process.
     Inductive ThreadGenStep : t -> option (t * TE) -> Prop :=
     | tstep_nil :
         ThreadGenStep p_dead None
-    | tstep_cons : forall req cont (rep : Reply req),
+    | tstep_cons : forall (req : Request) cont (rep : Reply req),
         ThreadGenStep (p_cont req cont)
                       (Some (cont rep, rep <~ req)).
 
@@ -119,143 +122,244 @@ Module Process.
     { gen_step := ThreadGenStep }.
   End defn.
 
-  (* Section tests. *)
-  (*   Import . *)
-
-  (*   Let PID := True. *)
-  (*   Let Handler := @Var.t PID nat. *)
-  (*   Let Req := get_handler_req_pid Handler. *)
-  (*   Let Rep := get_handler_ret_pid Handler. *)
-  (*   Let TE := @TraceElem PID Req Rep. *)
-
-  (*   Let my_prog : @Process _ Req Rep I := *)
-  (*     spawn I (do x <- Var.read; *)
-  (*              match x with *)
-  (*              | 0 => *)
-  (*                done Var.write 3 *)
-  (*              | _ => *)
-  (*                done Var.write 0 *)
-  (*              end). *)
-
-  (*   Local Ltac inv a := inversion a; subst; clear a. *)
-
-  (*   Goal forall t, *)
-  (*       GenEnsemble my_prog t -> *)
-  (*       exists x, *)
-  (*         t = [I @ 0 <~ Var.read; I @ I <~ Var.write 3] \/ *)
-  (*         t = [I @ x <~ Var.read; I @ I <~ Var.write 1]. *)
-  (*   Proof. *)
-  (*     intros. subst my_prog. *)
-  (*     inv H. *)
-  (*     - exfalso. inv H0. *)
-  (*     - inv H0. *)
-  (*   Abort. *)
-  (* End tests. *)
-End Process.
-
-Module Parallel.
-  Section defn.
-    Context {TE G__l G__r : Type} `{Generator TE G__l} `{Generator (ProcessEvent TE) G__r}.
-
-    Record Parallel :=
-      parallel
-        { gp_l : G__l;
-          gp_r : G__r
-        }.
-
-    Inductive ParallelStep : Parallel -> option (Parallel * (ProcessEvent TE)) -> Prop :=
-    | g_left : forall te g__l g__l' g__r,
-        g__l ~~> g__l' & te ->
-        ParallelStep (parallel g__l g__r) (Some (parallel g__l' g__r, 0 @ te))
-    | g_right : forall te pid g__l g__r g__r',
-        g__r ~~> g__r' & (pid @ te) ->
-        ParallelStep (parallel g__l g__r) (Some (parallel g__l g__r', S pid @ te))
-    | g_nil : forall g__l g__r,
-        g__l ~~>x ->
-        g__r ~~>x ->
-        ParallelStep (parallel g__l g__r) None.
-
-    Global Instance genPairGen : Generator (ProcessEvent TE) Parallel :=
-      { gen_step := ParallelStep }.
-
-    Definition wrap_singleton : list TE -> list (ProcessEvent TE) :=
-      map (fun e => 0 @ e).
-  End defn.
-
-  Infix "<||>" := parallel (right associativity, at level 101) : slot_scope.
-  Notation "[| |]" := (Empty.t) : slot_scope.
-  Notation "[| x |]" := (wrap_singleton x) : slot_scope.
-  Notation "[| x ; .. ; y ; z |]" := (parallel x (.. (parallel y (wrap_singleton z)) ..)) : slot_scope.
-
   Section tests.
-    (* Check that all interleavings created by the ensemble are valid: *)
-    Goal forall t,
-        GenEnsemble [| [1; 2]; [3] |] t ->
-        t = [0 @ 1; 0 @ 2; 1 @ 3] \/
-        t = [0 @ 1; 1 @ 3; 0 @ 2] \/
-        t = [1 @ 3; 0 @ 1; 0 @ 2].
-    Proof.
-      intros. sauto.
-    Qed.
+    Let Req := bool.
+    Let Rep req :=
+      match req with
+      | true => nat
+      | false => bool
+      end.
 
-    (* Check that it creates every interleaving: *)
-    Goal GenEnsemble [| [1; 2]; [3] |] [0 @ 1; 0 @ 2; 1 @ 3].
-    Proof.
-      constructor 2 with (g' := [| [2]; [3] |]).
-      - sauto.
-      - constructor 2 with (g' := [| []; [3] |]); sauto.
-    Qed.
+    Let my_prog : @Program Req Rep :=
+      do x <- true;
+      match x with
+      | 0 =>
+        done false
+      | _ =>
+        done true
+      end.
 
-    Goal GenEnsemble [| [1; 2]; [3] |] [0 @ 1; 1 @ 3; 0 @ 2].
-    Proof.
-      constructor 2 with (g' := [| [2]; [3] |]).
-      - sauto.
-      - constructor 2 with (g' := [| [2] ; [] |] ); sauto.
-    Qed.
-
-    Goal GenEnsemble [| [1; 2] ; [3] |] [1 @ 3; 0 @ 1; 0 @ 2].
-    Proof.
-      constructor 2 with (g' := [| [1; 2] ; [] |]).
-      - sauto.
-      - constructor 2 with (g' := [| [2] ; [] |]); sauto.
-    Qed.
+    Local Ltac inv a := inversion a; subst; clear a.
 
     Goal forall t,
-        GenEnsemble [| [3] ; [1; 2] |] t ->
-        t = [1 @ 1; 1 @ 2; 0 @ 3] \/
-        t = [1 @ 1; 0 @ 3; 1 @ 2] \/
-        t = [0 @ 3; 1 @ 1; 1 @ 2].
+        GenEnsemble my_prog t ->
+        exists x y z,
+          t = [0 <~ true; x <~ false] \/
+          t = [y <~ true; z <~ true].
     Proof.
-      intros. sauto.
-    Qed.
-
-    (* Test interleavings of larger system *)
-    Goal forall t,
-        GenEnsemble [| [1; 2]; [3; 4] |] t ->
-        t = [0 @ 1; 0 @ 2; 1 @ 3; 1 @ 4] \/
-        t = [0 @ 1; 1 @ 3; 0 @ 2; 1 @ 4] \/
-        t = [0 @ 1; 1 @ 3; 1 @ 4; 0 @ 2] \/
-
-        t = [1 @ 3; 0 @ 1; 0 @ 2; 1 @ 4] \/
-        t = [1 @ 3; 0 @ 1; 1 @ 4; 0 @ 2] \/
-        t = [1 @ 3; 1 @ 4; 0 @ 1; 0 @ 2].
-    Proof.
-      intros. sauto.
-    Qed.
-
-    (* Test interleavings of a system with 3 processes *)
-    Goal forall t,
-        GenEnsemble [| [0]; [1]; [2] |] t ->
-        t = [0 @ 0; 1 @ 1; 2 @ 2] \/
-        t = [0 @ 0; 2 @ 2; 1 @ 1] \/
-
-        t = [1 @ 1; 0 @ 0; 2 @ 2] \/
-        t = [1 @ 1; 2 @ 2; 0 @ 0] \/
-
-        t = [2 @ 2; 1 @ 1; 0 @ 0] \/
-        t = [2 @ 2; 0 @ 0; 1 @ 1].
-    Proof.
-      intros. sauto.
-    Qed.
+      intros. subst my_prog.
+      inv H.
+      - exfalso. inv H0.
+      - inv H0.
+    Abort.
   End tests.
-End Parallel.
+End process.
+
+Section parallel_defn.
+  Context {TE G__l G__r : Type} `{Generator TE G__l} `{Generator (ProcessEvent TE) G__r}.
+
+  Record Parallel :=
+    parallel
+      { gp_l : G__l;
+        gp_r : G__r
+      }.
+
+  Inductive ParallelStep : Parallel -> option (Parallel * (ProcessEvent TE)) -> Prop :=
+  | g_left : forall te g__l g__l' g__r,
+      g__l ~~> g__l' & te ->
+      ParallelStep (parallel g__l g__r) (Some (parallel g__l' g__r, 0 @ te))
+  | g_right : forall te pid g__l g__r g__r',
+      g__r ~~> g__r' & (pid @ te) ->
+      ParallelStep (parallel g__l g__r) (Some (parallel g__l g__r', S pid @ te))
+  | g_nil : forall g__l g__r,
+      g__l ~~>x ->
+      g__r ~~>x ->
+      ParallelStep (parallel g__l g__r) None.
+
+  Global Instance genPairGen : Generator (ProcessEvent TE) Parallel :=
+    { gen_step := ParallelStep }.
+
+  Definition wrap_singleton : list TE -> list (ProcessEvent TE) :=
+    map (fun e => 0 @ e).
+End parallel_defn.
+
+Infix "<||>" := parallel (right associativity, at level 101) : slot_scope.
+Notation "[| |]" := (Empty.t) : slot_scope.
+Notation "[| x |]" := (wrap_singleton x) : slot_scope.
+Notation "[| x ; .. ; y ; z |]" := (parallel x (.. (parallel y (wrap_singleton z)) ..)) : slot_scope.
+
+Section parallel_tests.
+  (* Check that all interleavings created by the ensemble are valid: *)
+  Goal forall t,
+      GenEnsemble [| [1; 2]; [3] |] t ->
+      t = [0 @ 1; 0 @ 2; 1 @ 3] \/
+      t = [0 @ 1; 1 @ 3; 0 @ 2] \/
+      t = [1 @ 3; 0 @ 1; 0 @ 2].
+  Proof.
+    intros. sauto.
+  Qed.
+
+  (* Check that it creates every interleaving: *)
+  Goal GenEnsemble [| [1; 2]; [3] |] [0 @ 1; 0 @ 2; 1 @ 3].
+  Proof.
+    constructor 2 with (g' := [| [2]; [3] |]).
+    - sauto.
+    - constructor 2 with (g' := [| []; [3] |]); sauto.
+  Qed.
+
+  Goal GenEnsemble [| [1; 2]; [3] |] [0 @ 1; 1 @ 3; 0 @ 2].
+  Proof.
+    constructor 2 with (g' := [| [2]; [3] |]).
+    - sauto.
+    - constructor 2 with (g' := [| [2] ; [] |] ); sauto.
+  Qed.
+
+  Goal GenEnsemble [| [1; 2] ; [3] |] [1 @ 3; 0 @ 1; 0 @ 2].
+  Proof.
+    constructor 2 with (g' := [| [1; 2] ; [] |]).
+    - sauto.
+    - constructor 2 with (g' := [| [2] ; [] |]); sauto.
+  Qed.
+
+  Goal forall t,
+      GenEnsemble [| [3] ; [1; 2] |] t ->
+      t = [1 @ 1; 1 @ 2; 0 @ 3] \/
+      t = [1 @ 1; 0 @ 3; 1 @ 2] \/
+      t = [0 @ 3; 1 @ 1; 1 @ 2].
+  Proof.
+    intros. sauto.
+  Qed.
+
+  (* Test interleavings of larger system *)
+  Goal forall t,
+      GenEnsemble [| [1; 2]; [3; 4] |] t ->
+      t = [0 @ 1; 0 @ 2; 1 @ 3; 1 @ 4] \/
+      t = [0 @ 1; 1 @ 3; 0 @ 2; 1 @ 4] \/
+      t = [0 @ 1; 1 @ 3; 1 @ 4; 0 @ 2] \/
+
+      t = [1 @ 3; 0 @ 1; 0 @ 2; 1 @ 4] \/
+      t = [1 @ 3; 0 @ 1; 1 @ 4; 0 @ 2] \/
+      t = [1 @ 3; 1 @ 4; 0 @ 1; 0 @ 2].
+  Proof.
+    intros. sauto.
+  Qed.
+
+  (* Test interleavings of a system with 3 processes *)
+  Goal forall t,
+      GenEnsemble [| [0]; [1]; [2] |] t ->
+      t = [0 @ 0; 1 @ 1; 2 @ 2] \/
+      t = [0 @ 0; 2 @ 2; 1 @ 1] \/
+
+      t = [1 @ 1; 0 @ 0; 2 @ 2] \/
+      t = [1 @ 1; 2 @ 2; 0 @ 0] \/
+
+      t = [2 @ 2; 1 @ 1; 0 @ 0] \/
+      t = [2 @ 2; 0 @ 0; 1 @ 1].
+  Proof.
+    intros. sauto.
+  Qed.
+End parallel_tests.
+
+From SLOT Require Import
+     Properties.
+
+From Coq Require Import
+     Classical_Prop.
+
+Section gen_commutativity.
+  Context {TE Gen} `{Generator (ProcessEvent TE) Gen}.
+
+  Definition generator_events_commute g :=
+    forall (p1 p2 : PID) (te1 te2 : TE) (g' g'' : Gen),
+    p1 <> p2 ->
+    g ~~> g' & (p1 @ te1) ->
+    g' ~~> g'' & (p2 @ te2) ->
+    exists g_,
+      g'' ~~> g_ & (p2 @ te2) \/ g_ ~~> g & (p1 @ te1).
+End gen_commutativity.
+
+(* Lemma gen_pair_comm {G1 G2 TE} `{Generator TE G1} `{Generator _ G2} (g1 : G1) (g2 : G2) : generator_events_commute (g1 <||> g2). *)
+(* Proof. *)
+(*   unfold generator_events_commute. intros *. intros Hpids Hg' Hg''. *)
+(*   inversion Hg'; subst. *)
+(*   -  *)
+
+Section optimize.
+  Context {Gen State Event : Type}.
+  Let TE := (ProcessEvent Event).
+  Context `{Hssp : StateSpace State TE} `{Hgen : Generator TE Gen}.
+
+  Let can_follow (te1 te2 : TE) : Prop :=
+    let (pid1, _) := te1 in
+    let (pid2, _) := te2 in
+    pid1 <= pid2 \/ not (events_commute te1 te2).
+
+  Inductive GenEnsembleOpt (g : Gen) : @TraceEnsemble TE :=
+  | og_ens_nil :
+      g  ~~>x ->
+      GenEnsembleOpt g []
+  | og_ens_first : forall g' te,
+      g  ~~> g' & te ->
+      g' ~~>x ->
+      GenEnsembleOpt g [te]
+  | og_ens_cons : forall g' te te' t,
+      g ~~> g' & te ->
+      can_follow te te' ->
+      GenEnsembleOpt g' (te' :: t) ->
+      GenEnsembleOpt g (te :: te' :: t).
+
+  Theorem optimize_gen_p g :
+    sufficient_replacement_p (GenEnsemble g) (GenEnsembleOpt g).
+  Admitted.
+
+  Theorem optimize_gen (g : Gen) P Q :
+    -{{ P }} GenEnsembleOpt g {{ Q }} ->
+    -{{ P }} GenEnsemble g {{ Q }}.
+  Proof.
+    apply ht_sufficient_replacement, comm_perm_sufficient_replacement, optimize_gen_p.
+  Qed.
+End optimize.
+
+Require Handlers.Deterministic.
+
+Section optimize_tests.
+  Import Deterministic.Var.
+
+  Let e (a : PID) (b : nat) : TraceElem var_req_t var_ret_t := a @ I <~ write b.
+
+  Goal forall t,
+      GenEnsembleOpt [| [I <~ write 3] ; [I <~ write 1; I <~ write 2] |] t ->
+      t = [1 @ I <~ write 1; 1 @ I <~ write 2; 0 @ I <~ write 3] \/
+      t = [1 @ I <~ write 1; 0 @ I <~ write 3; 1 @ I <~ write 2] \/
+      t = [0 @ I <~ write 3; 1 @ I <~ write 1; 1 @ I <~ write 2].
+  Proof.
+    intros. sauto.
+  Qed.
+
+  Hint Resolve var_ww_comm:slot.
+
+  (* Check that it creates every interleaving: *)
+  Goal GenEnsembleOpt [| [I <~ write 1; I <~ write 2]; [I <~ write 3] |]
+       [e 0 1; e 0 2; e 1 3].
+  Proof.
+    sauto db:slot.
+  Qed.
+
+  Goal GenEnsembleOpt [| [I <~ write 1; I <~ write 2]; [I <~ write 3] |]
+       [e 0 1; e 1 3; e 0 2].
+  Proof.
+    sauto use:var_ww_comm.
+    constructor 3 with (g' := [| [I <~ write 2]; [I <~ write 3] |]); try sauto.
+    - constructor 3 with (g' := [| [I <~ write 2]; [] |]); try sauto.
+      constructor 2; try sauto.
+      intros s s'.
+  Qed.
+
+
+  Goal GenEnsembleOpt [| [1; 2] ; [3] |] [1 @ 3; 0 @ 1; 0 @ 2].
+  Proof.
+    constructor 3 with (g' := [| [1; 2] ; [] |]).
+    - sauto.
+    - constructor 3 with (g' := [| [2] ; [] |]); sauto.
+  Qed.
+End optimize_tests.
