theories/Properties.v
@@ -13,12 +13,115 @@
    You should have received a copy of the GNU General Public License
    along with this program.  If not, see <https://www.gnu.org/licenses/>.
  *)
+From Coq Require Import
+     List
+     Relations.
+
+Import ListNotations.
+
 From SLOT Require Export
-     Foundations.
+     Foundations
+     Permutation
+     Commutativity
+     Tactics.
 
 Section defns.
-  Context `{StateSpace}.
+  Context `{Hssp : StateSpace}.
 
   Definition PossibleTrace t :=
     exists s s', ReachableByTrace s t s'.
+
+  (** [rbt_split] is an important observation that there is a point in
+  the state space for each intermediate step of the trace
+  execution: *)
+  Lemma rbt_split : forall s s'' t1 t2,
+      ReachableByTrace s (t1 ++ t2) s'' ->
+      exists s', ReachableByTrace s t1 s' /\ ReachableByTrace s' t2 s''.
+  Proof.
+    intros.
+    generalize dependent s.
+    induction t1; intros.
+    - exists s.
+      split; auto with slot.
+    - long_step H.
+      specialize (IHt1 s0 H).
+      destruct IHt1.
+      exists x. split.
+      + forward s0; firstorder.
+      + firstorder.
+  Qed.
+
+  (** [rbt_concat] lemma demonstrates that traces can be composed: *)
+  Lemma rbt_concat : forall s s' s'' t1 t2,
+      ReachableByTrace s t1 s' ->
+      ReachableByTrace s' t2 s'' ->
+      ReachableByTrace s (t1 ++ t2) s''.
+  Proof with auto.
+    intros.
+    generalize dependent s.
+    induction t1; intros; simpl...
+    - inversion H...
+    - long_step H.
+      forward s0...
+  Qed.
+
+  Lemma ht_comm_perm  s s' t t' :
+    ReachableByTrace s t s' ->
+    Permutation events_commute t t' ->
+    ReachableByTrace s t' s'.
+  Proof with eauto with slot.
+    intros Hls Hperm.
+    generalize dependent s.
+    induction Hperm; intros...
+    - long_step Hls.
+      forward s0...
+    - unfold_trace Hls.
+      specialize (H s s1).
+      replace (b :: a :: l) with ([b; a] ++ l) by reflexivity.
+      apply rbt_concat with (s' := s1)...
+      apply H.
+      forward s0...
+  Qed.
 End defns.
+
+Section ensemble_equiv.
+  Context `{StateSpace} (e1 e2 : TraceEnsemble Event).
+
+  Definition sufficient_replacement :=
+    forall t s s', e1 t ->
+              ReachableByTrace s t s' ->
+              exists t', e2 t' /\ ReachableByTrace s t' s'.
+
+  Definition sufficient_replacement_p :=
+    forall t, e1 t ->
+         exists t', e2 t' /\ Permutation events_commute t t'.
+
+  Theorem ht_sufficient_replacement P Q :
+    sufficient_replacement ->
+    -{{P}} e2 {{Q}} -> -{{P}} e1 {{Q}}.
+  Proof.
+    intros He2 Heht t Ht s s' Hls Hpre.
+    destruct (He2 t s s' Ht Hls) as [t' [Ht' Hls']].
+    eapply Heht; eauto.
+  Qed.
+
+  Lemma comm_perm_sufficient_replacement :
+    sufficient_replacement_p ->
+    sufficient_replacement.
+  Proof.
+    intros Hsrp t s s' Ht Hls.
+    destruct (Hsrp t Ht) as [t' [Ht' Hperm]].
+    eapply ht_comm_perm in Hperm; eauto.
+  Qed.
+End ensemble_equiv.
+
+Lemma sufficient_replacement_p_trans `{StateSpace} :
+  transitive (@TraceEnsemble Event) sufficient_replacement_p.
+Proof.
+  intros e1 e2 e3 H12 H23. intros t Ht.
+  apply H12 in Ht. destruct Ht as [t' [Ht' Hperm']].
+  apply H23 in Ht'. destruct Ht' as [t'' [Ht'' Hperm'']].
+  exists t''. split.
+  - assumption.
+  - eapply perm_trans; eauto.
+Qed.
